refactor(library/init/data): add fn_array
`fn_array A n` is defined as `fin n -> A`

In Lean, we currently don't have good support for using nested inductive
datatypes such as

   inductive Expr
   | app : string -> list Expr -> Expr
   | var : string -> Expr

The main issue is that users currently need to use well-founded
recursion to be able to define recursive functions over nested inductive
datatypes. Since the equation compiler does not have support for
well-founded recursion, this is a very laborious step.

This feature is needed in the KreMLin project.
So, I suggested they use the following workaround.

   inductive Expr
   | app : string -> forall n, fn_array Expr n -> Expr
   | var : string -> Expr

This is similar to the trick we used to use in the tactic framework.
Note that, `array Expr n` cannot be used because it would trigger the
nested inductive compiler.

After adding fn_array, I defined array on top of it.

Unfortunately, this change affected the hash_map module.
I repaired some of the broken lemmas, but we still have two broken ones.

library/init/data/array/basic.lean
@@ -4,56 +4,38 @@ Released under Apache 2.0 license as described in the file LICENSE.
 Authors: Leonardo de Moura, Mario Carneiro
 -/
 prelude
-import init.data.nat
+import init.data.fn_array.basic
 universes u w
 
 structure array (α : Type u) (n : nat) :=
-(data : fin n → α)
+(data : fn_array α n)
 
 def mk_array {α} (n) (v : α) : array α n :=
-{data := λ _, v}
+{data := mk_fn_array n v}
 
 namespace array
 variables {α : Type u} {β : Type w} {n : nat}
 
 def nil {α} : array α 0 :=
-{data := λ ⟨x, h⟩, absurd h (nat.not_lt_zero x)}
+{data := fn_array.nil}
 
 def read (a : array α n) (i : fin n) : α :=
-a.data i
+a.data.read i
 
 def read' [inhabited α] (a : array α n) (i : nat) : α :=
-if h : i < n then a.read ⟨i,h⟩ else default α
+a.data.read' i
 
 def write (a : array α n) (i : fin n) (v : α) : array α n :=
-{data := λ j, if i = j then v else a.read j}
+{data := a.data.write i v}
 
 def write' (a : array α n) (i : nat) (v : α) : array α n :=
-if h : i < n then a.write ⟨i, h⟩ v else a
-
-lemma push_back_idx {j n} (h₁ : j < n + 1) (h₂ : j ≠ n) : j < n :=
-nat.lt_of_le_and_ne (nat.le_of_lt_succ h₁) h₂
+{data := a.data.write' i v}
 
 def push_back (a : array α n) (v : α) : array α (n+1) :=
-{data := λ ⟨j, h₁⟩, if h₂ : j = n then v else a.read ⟨j, push_back_idx h₁ h₂⟩}
-
-lemma pop_back_idx {j n} (h : j < n) : j < n + 1 :=
-nat.lt.step h
+{data := a.data.push_back v}
 
 def pop_back (a : array α (n+1)) : array α n :=
-{data := λ ⟨j, h⟩, a.read ⟨j, pop_back_idx h⟩}
-
-lemma lt_aux_1 {a b c : nat} (h : a + c < b) : a < b :=
-lt_of_le_of_lt (nat.le_add_right a c) h
-
-lemma lt_aux_2 {n} (h : n > 0) : n - 1 < n :=
-have h₁ : 1 > 0, from dec_trivial,
-nat.sub_lt h h₁
-
-lemma lt_aux_3 {n i} (h : i + 1 < n) : n - 2 - i < n  :=
-have n > 0,     from lt.trans (nat.zero_lt_succ i) h,
-have n - 2 < n, from nat.sub_lt this (dec_trivial),
-lt_of_le_of_lt (nat.sub_le _ _) this
+{data := a.data.pop_back}
 
 @[elab_as_eliminator]
 theorem write_ind (a : array α n) (i : fin n) (v : α) (C : fin n → α → Sort w)
@@ -62,14 +44,8 @@ show C j (if i = j then v else read a j), from
 if h : i = j then by rwa [if_pos h, -h]
 else by rw [if_neg h]; exact Hj j h
 
-def foreach_aux (f : fin n → α → α) : Π (i : nat), i ≤ n → array α n → array α n
-| 0     h a := a
-| (j+1) h a :=
-  let i : fin n := ⟨n - 1 - j, nat.sub_one_sub_lt h⟩ in
-  foreach_aux j (le_of_lt h) (a.write i (f i (a.read i)))
-
 def foreach (a : array α n) (f : fin n → α → α) : array α n :=
-foreach_aux f n (le_refl _) a
+{data := a.data.foreach f}
 
 def map (f : α → α) (a : array α n) : array α n :=
 foreach a (λ _, f)
@@ -77,46 +53,34 @@ foreach a (λ _, f)
 def map₂ (f : α → α → α) (a b : array α n) : array α n :=
 foreach b (λ i, f (a.read i))
 
-def iterate_aux (a : array α n) (f : fin n → α → β → β) : Π (i : nat), i ≤ n → β → β
-| 0     h b := b
-| (j+1) h b :=
-  let i : fin n := ⟨j, h⟩ in
-  f i (a.read i) (iterate_aux j (le_of_lt h) b)
+def iterate_aux (a : array α n) (f : fin n → α → β → β) : Π (i : nat), i ≤ n → β → β :=
+a.data.iterate_aux f
 
 def iterate (a : array α n) (b : β) (fn : fin n → α → β → β) : β :=
-iterate_aux a fn n (le_refl _) b
+a.data.iterate b fn
 
 def foldl (a : array α n) (b : β) (f : α → β → β) : β :=
-iterate a b (λ _, f)
+a.data.foldl b f
 
 def rev_list (a : array α n) : list α :=
-a.foldl [] (λ v l, v :: l)
-
-def foldl_eq_aux (a : array α n) (b : β) (f : α → β → β) :
-  Π (i : nat) (h : i ≤ n), iterate_aux a (λ _, f) i h b = (iterate_aux a (λ _ v l, v :: l) i h []).foldr f b
-| 0     h := rfl
-| (j+1) h := congr_arg (f (read a ⟨j, h⟩)) (foldl_eq_aux j _)
+a.data.rev_list
 
 def foldl_eq (a : array α n) (b : β) (f : α → β → β) : a.foldl b f = a.rev_list.foldr f b :=
-foldl_eq_aux a b f _ _
-
-def rev_iterate_aux (a : array α n) (f : fin n → α → β → β) : Π (i : nat), i ≤ n → β → β
-| 0     h b := b
-| (j+1) h b :=
-  let i : fin n := ⟨j, h⟩ in
-  rev_iterate_aux j (le_of_lt h) (f i (a.read i) b)
+by cases a; apply fn_array.foldl_eq
 
 def rev_iterate (a : array α n) (b : β) (fn : fin n → α → β → β) : β :=
-rev_iterate_aux a fn n (le_refl _) b
+a.data.rev_iterate b fn
 
 def to_list (a : array α n) : list α :=
-a.rev_iterate [] (λ _ v l, v :: l)
+a.data.to_list
 
-protected def mem (v : α) (a : array α n) : Prop := ∃i, read a i = v
+protected def mem (v : α) (a : array α n) : Prop :=
+a.data.mem v
 
 instance : has_mem α (array α n) := ⟨array.mem⟩
 
-theorem read_mem (a : array α n) (i) : read a i ∈ a := exists.intro i rfl
+theorem read_mem (a : array α n) (i) : read a i ∈ a :=
+exists.intro i rfl
 
 instance [has_to_string α] : has_to_string (array α n) :=
 ⟨to_string ∘ to_list⟩
@@ -130,4 +94,4 @@ meta instance [has_to_tactic_format α] : has_to_tactic_format (array α n) :=
 end array
 
 def list.to_array {α} (l : list α) : array α l.length :=
-{data := λ v, l.nth_le v.1 v.2}
+{data := list.to_fn_array l}
