library/init/data/fn_array/basic.lean
@@ -1,0 +1,134 @@
+/-
+Copyright (c) 2017 Microsoft Corporation. All rights reserved.
+Released under Apache 2.0 license as described in the file LICENSE.
+Authors: Leonardo de Moura, Mario Carneiro
+-/
+prelude
+import init.data.nat
+universes u w
+
+def fn_array (α : Type u) (n : nat) :=
+fin n → α
+
+def mk_fn_array {α} (n) (v : α) : fn_array α n :=
+λ _, v
+
+namespace fn_array
+variables {α : Type u} {β : Type w} {n : nat}
+
+def nil {α} : fn_array α 0 :=
+λ ⟨x, h⟩, absurd h (nat.not_lt_zero x)
+
+def read (a : fn_array α n) (i : fin n) : α :=
+a i
+
+def read' [inhabited α] (a : fn_array α n) (i : nat) : α :=
+if h : i < n then a.read ⟨i,h⟩ else default α
+
+def write (a : fn_array α n) (i : fin n) (v : α) : fn_array α n :=
+λ j, if i = j then v else a.read j
+
+def write' (a : fn_array α n) (i : nat) (v : α) : fn_array α n :=
+if h : i < n then a.write ⟨i, h⟩ v else a
+
+lemma push_back_idx {j n} (h₁ : j < n + 1) (h₂ : j ≠ n) : j < n :=
+nat.lt_of_le_and_ne (nat.le_of_lt_succ h₁) h₂
+
+def push_back (a : fn_array α n) (v : α) : fn_array α (n+1) :=
+λ ⟨j, h₁⟩, if h₂ : j = n then v else a.read ⟨j, push_back_idx h₁ h₂⟩
+
+lemma pop_back_idx {j n} (h : j < n) : j < n + 1 :=
+nat.lt.step h
+
+def pop_back (a : fn_array α (n+1)) : fn_array α n :=
+λ ⟨j, h⟩, a.read ⟨j, pop_back_idx h⟩
+
+lemma lt_aux_1 {a b c : nat} (h : a + c < b) : a < b :=
+lt_of_le_of_lt (nat.le_add_right a c) h
+
+lemma lt_aux_2 {n} (h : n > 0) : n - 1 < n :=
+have h₁ : 1 > 0, from dec_trivial,
+nat.sub_lt h h₁
+
+lemma lt_aux_3 {n i} (h : i + 1 < n) : n - 2 - i < n  :=
+have n > 0,     from lt.trans (nat.zero_lt_succ i) h,
+have n - 2 < n, from nat.sub_lt this (dec_trivial),
+lt_of_le_of_lt (nat.sub_le _ _) this
+
+@[elab_as_eliminator]
+theorem write_ind (a : fn_array α n) (i : fin n) (v : α) (C : fin n → α → Sort w)
+  (Hi : C i v) (Hj : ∀j, i ≠ j → C j (a.read j)) (j) : C j ((a.write i v).read j) :=
+show C j (if i = j then v else read a j), from
+if h : i = j then by rwa [if_pos h, -h]
+else by rw [if_neg h]; exact Hj j h
+
+def foreach_aux (f : fin n → α → α) : Π (i : nat), i ≤ n → fn_array α n → fn_array α n
+| 0     h a := a
+| (j+1) h a :=
+  let i : fin n := ⟨n - 1 - j, nat.sub_one_sub_lt h⟩ in
+  foreach_aux j (le_of_lt h) (a.write i (f i (a.read i)))
+
+def foreach (a : fn_array α n) (f : fin n → α → α) : fn_array α n :=
+foreach_aux f n (le_refl _) a
+
+def map (f : α → α) (a : fn_array α n) : fn_array α n :=
+foreach a (λ _, f)
+
+def map₂ (f : α → α → α) (a b : fn_array α n) : fn_array α n :=
+foreach b (λ i, f (a.read i))
+
+def iterate_aux (a : fn_array α n) (f : fin n → α → β → β) : Π (i : nat), i ≤ n → β → β
+| 0     h b := b
+| (j+1) h b :=
+  let i : fin n := ⟨j, h⟩ in
+  f i (a.read i) (iterate_aux j (le_of_lt h) b)
+
+def iterate (a : fn_array α n) (b : β) (fn : fin n → α → β → β) : β :=
+iterate_aux a fn n (le_refl _) b
+
+def foldl (a : fn_array α n) (b : β) (f : α → β → β) : β :=
+iterate a b (λ _, f)
+
+def rev_list (a : fn_array α n) : list α :=
+a.foldl [] (λ v l, v :: l)
+
+theorem foldl_eq_aux (a : fn_array α n) (b : β) (f : α → β → β) :
+  Π (i : nat) (h : i ≤ n), iterate_aux a (λ _, f) i h b = (iterate_aux a (λ _ v l, v :: l) i h []).foldr f b
+| 0     h := rfl
+| (j+1) h := congr_arg (f (read a ⟨j, h⟩)) (foldl_eq_aux j _)
+
+theorem foldl_eq (a : fn_array α n) (b : β) (f : α → β → β) : a.foldl b f = a.rev_list.foldr f b :=
+foldl_eq_aux a b f _ _
+
+def rev_iterate_aux (a : fn_array α n) (f : fin n → α → β → β) : Π (i : nat), i ≤ n → β → β
+| 0     h b := b
+| (j+1) h b :=
+  let i : fin n := ⟨j, h⟩ in
+  rev_iterate_aux j (le_of_lt h) (f i (a.read i) b)
+
+def rev_iterate (a : fn_array α n) (b : β) (fn : fin n → α → β → β) : β :=
+rev_iterate_aux a fn n (le_refl _) b
+
+def to_list (a : fn_array α n) : list α :=
+a.rev_iterate [] (λ _ v l, v :: l)
+
+protected def mem (v : α) (a : fn_array α n) : Prop := ∃i, read a i = v
+
+instance : has_mem α (fn_array α n) := ⟨fn_array.mem⟩
+
+theorem read_mem (a : fn_array α n) (i) : read a i ∈ a :=
+exists.intro i rfl
+
+instance [has_to_string α] : has_to_string (fn_array α n) :=
+⟨to_string ∘ to_list⟩
+
+meta instance [has_to_format α] : has_to_format (fn_array α n) :=
+⟨to_fmt ∘ to_list⟩
+
+meta instance [has_to_tactic_format α] : has_to_tactic_format (fn_array α n) :=
+⟨tactic.pp ∘ to_list⟩
+
+end fn_array
+
+def list.to_fn_array {α} (l : list α) : fn_array α l.length :=
+λ v, l.nth_le v.1 v.2
